Dafny/examples/Challenge8/Challenge8CodeNEW.s.dfy
@@ -5,6 +5,7 @@ include "../../LLVM/behaviorLemmas.i.dfy"
 include "../../Libraries/Seqs.s.dfy"
 include "../../LLVM/memory.i.dfy"
 
+
 module challenge8CodeNEW{
     import opened control_flow
     import opened LLVM_def_NEW
@@ -18,16 +19,49 @@ module challenge8CodeNEW{
 //     Block([prefixCode(), Block([CNil]),postfixCode()])
 // }
 
-function challenge_8_transport_handler_create_conn_vuln_test():code {
-    Block([prefixCode(), Block([CNil]),postfixCode()])
+function allVariablesConfig():configuration
+{
+    var var_11 := LV("var_11");
+    var var_num_packets := LV("var_num_packets");
+    var var_conv15 := LV("var_conv15");
+    var var_12 := LV("var_12");
+    var var_size_addr := LV("var_size_addr");
+    var var_conv16 := LV("var_conv16");
+    var var_div := LV("var_div");
+    var var_cmp17 := LV("var_cmp17");
+    var var_call20 := LV("var_call20");
+    var var_retval := LV("var_retval");
+    var var_26 := LV("var_26");
+    var var_size := LV("var_size");
+    Config(map["var_11" := var_11,
+            "var_num_packets" := var_num_packets,
+            "var_conv15" := var_conv15,
+            "var_12" := var_12,
+            "var_size_addr" := var_size_addr,
+            "var_conv16" := var_conv16,
+            "var_div" := var_div,
+            "var_cmp17" := var_cmp17,
+            "var_call20" := var_call20,
+            "var_retval" := var_retval,
+            "var_26" := var_26,
+            "var_size" := var_size])
+}
+
+predicate validConfig(s:state,c:configuration)
+{
+    forall op :: op in c.ops ==> ValidOperand(s,c.ops[op])
+}
+
+function challenge_8_transport_handler_create_conn_vuln_test():seq<Code> {
+    [prefixCode(), Block([CNil]),postfixCode()]
 }
 //  Block([prefixCode(),patch_block,postfix])
 
-function prefixCode():code{
+function prefixCode():Code{
     Block([CNil])
 }
 
-function postfixCode():code{
+function postfixCode():Code{
     Block([CNil])
 }
 
@@ -70,171 +104,232 @@ function postfixCode():code{
 
 //     patch_block
 // }
-// function challenge_8_transport_handler_create_conn_patch():codeRe {
+function return_():Code{
+    var config := allVariablesConfig();
+    
+    var return_ := 
+    Block(
+        [Ins(LOAD(config.ops["var_26"],1,config.ops["var_retval"])),
+        Ins(RET(config.ops["var_26"]))]);
+    
+    return_
 
-//     // var num_packets := LV(" num_packets ");
-//     // var size := LV(" size ");
-//         //     ; Function Attrs: noinline nounwind optnone uwtable
-//         // define internal zeroext i8 @create_conn(i16 zeroext %size) #0 {
-//         // entry:
-//         //   %retval = alloca i8, align 1
-//         //   %size.addr = alloca i16, align 2
-//         //   store i16 %size, i16* %size.addr, align 2
-//         //   %0 = load i8, i8* @src, align 1
-//         //   %idxprom = zext i8 %0 to i64
-//         //   %arrayidx = getelementptr inbounds [256 x %struct.ConnectionInfo*], [256 x %struct.ConnectionInfo*]* @connection_infos, i64 0, i64 %idxprom
-//         //   %1 = load %struct.ConnectionInfo*, %struct.ConnectionInfo** %arrayidx, align 8
-//         //   %cmp = icmp eq %struct.ConnectionInfo* %1, null
-//         //   br i1 %cmp, label %if.then, label %if.end
+}
 
-//         // if.then:                                          ; preds = %entry
-//         //   %call = call noalias align 16 i8* @calloc(i64 1, i64 16) #9
-//         //   %2 = bitcast i8* %call to %struct.ConnectionInfo*
-//         //   %3 = load i8, i8* @src, align 1
-//         //   %idxprom1 = zext i8 %3 to i64
-//         //   %arrayidx2 = getelementptr inbounds [256 x %struct.ConnectionInfo*], [256 x %struct.ConnectionInfo*]* @connection_infos, i64 0, i64 %idxprom1
-//         //   store %struct.ConnectionInfo* %2, %struct.ConnectionInfo** %arrayidx2, align 8
-//         //   %4 = load i8, i8* @src, align 1
-//         //   %idxprom3 = zext i8 %4 to i64
-//         //   %arrayidx4 = getelementptr inbounds [256 x %struct.ConnectionInfo*], [256 x %struct.ConnectionInfo*]* @connection_infos, i64 0, i64 %idxprom3
-//         //   %5 = load %struct.ConnectionInfo*, %struct.ConnectionInfo** %arrayidx4, align 8
-//         //   %state = getelementptr inbounds %struct.ConnectionInfo, %struct.ConnectionInfo* %5, i32 0, i32 0
-//         //   store i32 0, i32* %state, align 8
-//         //   %6 = load i8, i8* @src, align 1
-//         //   %idxprom5 = zext i8 %6 to i64
-//         //   %arrayidx6 = getelementptr inbounds [256 x %struct.ConnectionInfo*], [256 x %struct.ConnectionInfo*]* @connection_infos, i64 0, i64 %idxprom5
-//         //   %7 = load %struct.ConnectionInfo*, %struct.ConnectionInfo** %arrayidx6, align 8
-//         //   %data = getelementptr inbounds %struct.ConnectionInfo, %struct.ConnectionInfo* %7, i32 0, i32 3
-//         //   store i8* null, i8** %data, align 8
-//         //   br label %if.end
+lemma returntest(s:state)
+   requires ValidState(s);
+    requires validStartingState(s)
+    requires validConfig(s,allVariablesConfig());
+{
+    var config := allVariablesConfig();
 
-//         // if.end:                                           ; preds = %if.then, %entry
-//         //   %8 = load i16, i16* %size.addr, align 2
-//         //   %conv = zext i16 %8 to i32
-//         //   %rem = srem i32 %conv, 7
-//         //   %cmp7 = icmp ne i32 %rem, 0
-//         //   br i1 %cmp7, label %if.then9, label %if.end14
-
-//         // if.then9:                                         ; preds = %if.end
-//         //   %9 = load i16, i16* %size.addr, align 2
-//         //   %conv10 = zext i16 %9 to i32
-//         //   %add = add nsw i32 %conv10, 7
-//         //   %10 = load i16, i16* %size.addr, align 2
-//         //   %conv11 = zext i16 %10 to i32
-//         //   %rem12 = srem i32 %conv11, 7
-//         //   %sub = sub nsw i32 %add, %rem12
-//         //   %conv13 = trunc i32 %sub to i16
-//         //   store i16 %conv13, i16* %size.addr, align 2
-//         //   br label %if.end14
-
-//     // var prefix := Block([]);
-
-//         //     if.end14:                                         ; preds = %if.then9, %if.end
-//         //   %11 = load i8, i8* @num_packets, align 1
-//         //   %conv15 = zext i8 %11 to i32
-//         //   %12 = load i16, i16* %size.addr, align 2
-//         //   %conv16 = zext i16 %12 to i32
-//         //   %div = sdiv i32 %conv16, 7
-//         //   %cmp17 = icmp sgt i32 %conv15, %div
-//         //   br i1 %cmp17, label %if.then19, label %if.end21
-
-//         // if.then19:                                        ; preds = %if.end14
-//         //   %call20 = call i32 (i8*, ...) @printf(i8* getelementptr inbounds ([44 x i8], [44 x i8]* @.str.6, i64 0, i64 0))
-//         //   call void @delete_connection()
-//         //   store i8 0, i8* %retval, align 1
-//         //   br label %return
-
-//     var postfix := postfixCode();
-
-//     var var_11 := LV(" var_11 ");
-//     var var_num_packets := LV(" var_num_packets ");
-//     var var_conv15 := LV(" var_conv15 ");
-//     var var_12 := LV(" var_12 ");
-//     var var_size_addr := LV(" var_size_addr ");
-//     var var_conv16 := LV(" var_conv16 ");
-//     var var_div := LV(" var_div ");
-//     var var_cmp17 := LV(" var_cmp17 ");
-//     var var_call20 := LV(" var_call20 ");
-//     var var_retval := LV(" var_retval ");
-//     var var_26 := LV(" var_26 ");
-//     var var_size := LV("var_size");
+    var b := [s] + evalCodeFn(return_(),s);
+    // assert s == b[0];
+    assert StateNext(b[0],b[1]);
+    // assert ValidState(b[1]);
 
 
+    // assert evalCodeFn(return_(),s) == evalCodeSeqFn(return_().block,s); 
+    // assert evalCodeSeqFn(return_().block,s) == evalCodeFn(first(return_().block),s) + evalCodeSeqFn(all_but_first(return_().block),last(evalCodeFn(first(return_().block),s)));
+    // var rest := evalCodeSeqFn(all_but_first(return_().block),last(evalCodeFn(first(return_().block),s)));
+    // assert first(return_().block).Ins?; 
+    // assert evalCodeFn(first(return_().block),s) == [evalInsRe(first(return_().block).ins,s)];
+    assert ValidState(b[1]);
+    assert ValidState(b[2]);
+    assert ValidState(b[3]);
+    assert |b| == 4;
+    assert NextStep(b[0],b[1],evalInsStep((LOAD(config.ops["var_26"],1,config.ops["var_retval"]))));
+    assert NextStep(b[1],b[2],evalInsStep((RET(config.ops["var_26"]))));
+    assert NextStep(b[2],b[3],Step.stutterStep());
 
-//     var return_ := Block([Ins(LOAD(var_26,1,var_retval)),
-//     Ins(RET(var_26))]);
+    // asser t
+    // assert b[1] == evalInsRe(first(return_().block).ins,s);
+    // assert b[1].ok ==> NextStep(b[0],b[1],Step.evalInsStep(first(return_().block).ins));
+    if(b[1].ok){
+        // assert NextStep(b[0],b[1],Step.evalInsStep(first(return_().block).ins));
+        assert exists step :: NextStep(b[0],b[1],step);
+        var step :| NextStep(b[0],b[1],step);
+        assert ValidState(b[0]);
+        assert ValidState(b[1]);
+        // assert b[0] != b[1];
+        assert step.evalInsStep?;
+    }
+    
+           assert exists step' :: NextStep(b[1],b[2],step');
+        var step' :| NextStep(b[1],b[2],step');
+        assert ValidState(b[1]);
+        assert ValidState(b[2]);
+        // assert b[0] != b[1];
+        assert step'.evalInsStep?;
+    // assert NextStep(b[0],b[1],evalInsStep((LOAD(config.ops["var_26"],1,config.ops["var_retval"]))));
+}
 
-//     // 
-//     var if_then19 := Block([Ins(CALL(D(Void),delete_connection())),
-//     Ins(STORE(D(Int(0,IntType(1,false))),var_retval)),
-//     Ins(UNCONDBR(return_))]);
+function if_then19():Code {
+        // 
+    var config := allVariablesConfig();
+    var if_then19 := Block([Ins(CALL(D(Void),delete_connection())),
+    Ins(STORE(D(Int(0,IntType(1,false))),config.ops["var_retval"])),
+    return_()]); // UNCONDBR is just converted to Block
+    if_then19
+}
 
-//     // var patch_block := Block([Ins(LOAD(var_11,1,var_num_packets)),
-//     // Ins(ZEXT(var_conv15,1,var_11,4)),
-//     // Ins(LOAD(var_12,2,var_size_addr)),
-//     // Ins(ZEXT(var_conv16,2,var_12,4)),
-//     // Ins(SDIV(var_div,var_conv16,D(Int(7,IntType(4,false))))),
-//     // Ins(ICMP(var_cmp17,sgt,4,var_conv15,var_div)),
-//     // Ins(BR(var_cmp17,if_then19,postfix))]);
+function challenge_8_transport_handler_create_conn_patch():seq<Code>  {
+
+    // var num_packets := LV(" num_packets ");
+    // var size := LV(" size ");
+        //     ; Function Attrs: noinline nounwind optnone uwtable
+        // define internal zeroext i8 @create_conn(i16 zeroext %size) #0 {
+        // entry:
+        //   %retval = alloca i8, align 1
+        //   %size.addr = alloca i16, align 2
+        //   store i16 %size, i16* %size.addr, align 2
+        //   %0 = load i8, i8* @src, align 1
+        //   %idxprom = zext i8 %0 to i64
+        //   %arrayidx = getelementptr inbounds [256 x %struct.ConnectionInfo*], [256 x %struct.ConnectionInfo*]* @connection_infos, i64 0, i64 %idxprom
+        //   %1 = load %struct.ConnectionInfo*, %struct.ConnectionInfo** %arrayidx, align 8
+        //   %cmp = icmp eq %struct.ConnectionInfo* %1, null
+        //   br i1 %cmp, label %if.then, label %if.end
+
+        // if.then:                                          ; preds = %entry
+        //   %call = call noalias align 16 i8* @calloc(i64 1, i64 16) #9
+        //   %2 = bitcast i8* %call to %struct.ConnectionInfo*
+        //   %3 = load i8, i8* @src, align 1
+        //   %idxprom1 = zext i8 %3 to i64
+        //   %arrayidx2 = getelementptr inbounds [256 x %struct.ConnectionInfo*], [256 x %struct.ConnectionInfo*]* @connection_infos, i64 0, i64 %idxprom1
+        //   store %struct.ConnectionInfo* %2, %struct.ConnectionInfo** %arrayidx2, align 8
+        //   %4 = load i8, i8* @src, align 1
+        //   %idxprom3 = zext i8 %4 to i64
+        //   %arrayidx4 = getelementptr inbounds [256 x %struct.ConnectionInfo*], [256 x %struct.ConnectionInfo*]* @connection_infos, i64 0, i64 %idxprom3
+        //   %5 = load %struct.ConnectionInfo*, %struct.ConnectionInfo** %arrayidx4, align 8
+        //   %state = getelementptr inbounds %struct.ConnectionInfo, %struct.ConnectionInfo* %5, i32 0, i32 0
+        //   store i32 0, i32* %state, align 8
+        //   %6 = load i8, i8* @src, align 1
+        //   %idxprom5 = zext i8 %6 to i64
+        //   %arrayidx6 = getelementptr inbounds [256 x %struct.ConnectionInfo*], [256 x %struct.ConnectionInfo*]* @connection_infos, i64 0, i64 %idxprom5
+        //   %7 = load %struct.ConnectionInfo*, %struct.ConnectionInfo** %arrayidx6, align 8
+        //   %data = getelementptr inbounds %struct.ConnectionInfo, %struct.ConnectionInfo* %7, i32 0, i32 3
+        //   store i8* null, i8** %data, align 8
+        //   br label %if.end
+
+        // if.end:                                           ; preds = %if.then, %entry
+        //   %8 = load i16, i16* %size.addr, align 2
+        //   %conv = zext i16 %8 to i32
+        //   %rem = srem i32 %conv, 7
+        //   %cmp7 = icmp ne i32 %rem, 0
+        //   br i1 %cmp7, label %if.then9, label %if.end14
+
+        // if.then9:                                         ; preds = %if.end
+        //   %9 = load i16, i16* %size.addr, align 2
+        //   %conv10 = zext i16 %9 to i32
+        //   %add = add nsw i32 %conv10, 7
+        //   %10 = load i16, i16* %size.addr, align 2
+        //   %conv11 = zext i16 %10 to i32
+        //   %rem12 = srem i32 %conv11, 7
+        //   %sub = sub nsw i32 %add, %rem12
+        //   %conv13 = trunc i32 %sub to i16
+        //   store i16 %conv13, i16* %size.addr, align 2
+        //   br label %if.end14
+
+    // var prefix := Block([]);
+
+        //     if.end14:                                         ; preds = %if.then9, %if.end
+        //   %11 = load i8, i8* @num_packets, align 1
+        //   %conv15 = zext i8 %11 to i32
+        //   %12 = load i16, i16* %size.addr, align 2
+        //   %conv16 = zext i16 %12 to i32
+        //   %div = sdiv i32 %conv16, 7
+        //   %cmp17 = icmp sgt i32 %conv15, %div
+        //   br i1 %cmp17, label %if.then19, label %if.end21
+
+        // if.then19:                                        ; preds = %if.end14
+        //   %call20 = call i32 (i8*, ...) @printf(i8* getelementptr inbounds ([44 x i8], [44 x i8]* @.str.6, i64 0, i64 0))
+        //   call void @delete_connection()
+        //   store i8 0, i8* %retval, align 1
+        //   br label %return
+
+    // var postfix := postfixCode();
+
+    // var var_11 := LV("var_11");
+    // var var_num_packets := LV("var_num_packets");
+    // var var_conv15 := LV("var_conv15");
+    // var var_12 := LV("var_12");
+    // var var_size_addr := LV("var_size_addr");
+    // var var_conv16 := LV("var_conv16");
+    // var var_div := LV("var_div");
+    // var var_cmp17 := LV("var_cmp17");
+    // var var_call20 := LV("var_call20");
+    // // var var_retval := LV("var_retval");
+    // var var_26 := LV("var_26");
+    // var var_size := LV("var_size");
+    var config := allVariablesConfig();
+
+    // var patch_block := Block([Ins(LOAD(var_11,1,var_num_packets)),
+    // Ins(ZEXT(var_conv15,1,var_11,4)),
+    // Ins(LOAD(var_12,2,var_size_addr)),
+    // Ins(ZEXT(var_conv16,2,var_12,4)),
+    // Ins(SDIV(var_div,var_conv16,D(Int(7,IntType(4,false))))),
+    // Ins(ICMP(var_cmp17,sgt,4,var_conv15,var_div)),
+    // Ins(BR(var_cmp17,if_then19,postfix))]);
 
     
-//     var patch_block := Block([Ins(SDIV(var_div,var_size,D(Int(7,IntType(4,false))))),
-//     Ins(ICMP(var_cmp17,sgt,4,var_num_packets,var_div)),
-//     Ins(BR(var_cmp17,if_then19,postfix))]);
+    var patch_block := 
+    Block([Ins(SDIV(config.ops["var_div"],config.ops["var_size"],D(Int(7,IntType(4,false))))),
+    Ins(ICMP(config.ops["var_cmp17"],sgt,4,config.ops["var_num_packets"],config.ops["var_div"])),
+    IfElse(config.ops["var_cmp17"],if_then19(),postfixCode())]);
 
-//         //         if.end21:                                         ; preds = %if.end14
-//         //   %13 = load i8, i8* @src, align 1
-//         //   %idxprom22 = zext i8 %13 to i64
-//         //   %arrayidx23 = getelementptr inbounds [256 x %struct.ConnectionInfo*], [256 x %struct.ConnectionInfo*]* @connection_infos, i64 0, i64 %idxprom22
-//         //   %14 = load %struct.ConnectionInfo*, %struct.ConnectionInfo** %arrayidx23, align 8
-//         //   %data24 = getelementptr inbounds %struct.ConnectionInfo, %struct.ConnectionInfo* %14, i32 0, i32 3
-//         //   %15 = load i8*, i8** %data24, align 8
-//         //   %cmp25 = icmp eq i8* %15, null
-//         //   br i1 %cmp25, label %if.then27, label %if.else
+        //         if.end21:                                         ; preds = %if.end14
+        //   %13 = load i8, i8* @src, align 1
+        //   %idxprom22 = zext i8 %13 to i64
+        //   %arrayidx23 = getelementptr inbounds [256 x %struct.ConnectionInfo*], [256 x %struct.ConnectionInfo*]* @connection_infos, i64 0, i64 %idxprom22
+        //   %14 = load %struct.ConnectionInfo*, %struct.ConnectionInfo** %arrayidx23, align 8
+        //   %data24 = getelementptr inbounds %struct.ConnectionInfo, %struct.ConnectionInfo* %14, i32 0, i32 3
+        //   %15 = load i8*, i8** %data24, align 8
+        //   %cmp25 = icmp eq i8* %15, null
+        //   br i1 %cmp25, label %if.then27, label %if.else
 
-//         // if.then27:                                        ; preds = %if.end21
-//         //   %16 = load i16, i16* %size.addr, align 2
-//         //   %conv28 = zext i16 %16 to i64
-//         //   %call29 = call noalias align 16 i8* @calloc(i64 %conv28, i64 1) #9
-//         //   %17 = load i8, i8* @src, align 1
-//         //   %idxprom30 = zext i8 %17 to i64
-//         //   %arrayidx31 = getelementptr inbounds [256 x %struct.ConnectionInfo*], [256 x %struct.ConnectionInfo*]* @connection_infos, i64 0, i64 %idxprom30
-//         //   %18 = load %struct.ConnectionInfo*, %struct.ConnectionInfo** %arrayidx31, align 8
-//         //   %data32 = getelementptr inbounds %struct.ConnectionInfo, %struct.ConnectionInfo* %18, i32 0, i32 3
-//         //   store i8* %call29, i8** %data32, align 8
-//         //   br label %if.end41
+        // if.then27:                                        ; preds = %if.end21
+        //   %16 = load i16, i16* %size.addr, align 2
+        //   %conv28 = zext i16 %16 to i64
+        //   %call29 = call noalias align 16 i8* @calloc(i64 %conv28, i64 1) #9
+        //   %17 = load i8, i8* @src, align 1
+        //   %idxprom30 = zext i8 %17 to i64
+        //   %arrayidx31 = getelementptr inbounds [256 x %struct.ConnectionInfo*], [256 x %struct.ConnectionInfo*]* @connection_infos, i64 0, i64 %idxprom30
+        //   %18 = load %struct.ConnectionInfo*, %struct.ConnectionInfo** %arrayidx31, align 8
+        //   %data32 = getelementptr inbounds %struct.ConnectionInfo, %struct.ConnectionInfo* %18, i32 0, i32 3
+        //   store i8* %call29, i8** %data32, align 8
+        //   br label %if.end41
 
-//         // if.else:                                          ; preds = %if.end21
-//         //   %19 = load i8, i8* @src, align 1
-//         //   %idxprom33 = zext i8 %19 to i64
-//         //   %arrayidx34 = getelementptr inbounds [256 x %struct.ConnectionInfo*], [256 x %struct.ConnectionInfo*]* @connection_infos, i64 0, i64 %idxprom33
-//         //   %20 = load %struct.ConnectionInfo*, %struct.ConnectionInfo** %arrayidx34, align 8
-//         //   %data35 = getelementptr inbounds %struct.ConnectionInfo, %struct.ConnectionInfo* %20, i32 0, i32 3
-//         //   %21 = load i8*, i8** %data35, align 8
-//         //   %22 = load i16, i16* %size.addr, align 2
-//         //   %conv36 = zext i16 %22 to i64
-//         //   %call37 = call align 16 i8* @realloc(i8* %21, i64 %conv36) #9
-//         //   %23 = load i8, i8* @src, align 1
-//         //   %idxprom38 = zext i8 %23 to i64
-//         //   %arrayidx39 = getelementptr inbounds [256 x %struct.ConnectionInfo*], [256 x %struct.ConnectionInfo*]* @connection_infos, i64 0, i64 %idxprom38
-//         //   %24 = load %struct.ConnectionInfo*, %struct.ConnectionInfo** %arrayidx39, align 8
-//         //   %data40 = getelementptr inbounds %struct.ConnectionInfo, %struct.ConnectionInfo* %24, i32 0, i32 3
-//         //   store i8* %call37, i8** %data40, align 8
-//         //   br label %if.end41
+        // if.else:                                          ; preds = %if.end21
+        //   %19 = load i8, i8* @src, align 1
+        //   %idxprom33 = zext i8 %19 to i64
+        //   %arrayidx34 = getelementptr inbounds [256 x %struct.ConnectionInfo*], [256 x %struct.ConnectionInfo*]* @connection_infos, i64 0, i64 %idxprom33
+        //   %20 = load %struct.ConnectionInfo*, %struct.ConnectionInfo** %arrayidx34, align 8
+        //   %data35 = getelementptr inbounds %struct.ConnectionInfo, %struct.ConnectionInfo* %20, i32 0, i32 3
+        //   %21 = load i8*, i8** %data35, align 8
+        //   %22 = load i16, i16* %size.addr, align 2
+        //   %conv36 = zext i16 %22 to i64
+        //   %call37 = call align 16 i8* @realloc(i8* %21, i64 %conv36) #9
+        //   %23 = load i8, i8* @src, align 1
+        //   %idxprom38 = zext i8 %23 to i64
+        //   %arrayidx39 = getelementptr inbounds [256 x %struct.ConnectionInfo*], [256 x %struct.ConnectionInfo*]* @connection_infos, i64 0, i64 %idxprom38
+        //   %24 = load %struct.ConnectionInfo*, %struct.ConnectionInfo** %arrayidx39, align 8
+        //   %data40 = getelementptr inbounds %struct.ConnectionInfo, %struct.ConnectionInfo* %24, i32 0, i32 3
+        //   store i8* %call37, i8** %data40, align 8
+        //   br label %if.end41
 
-//         // if.end41:                                         ; preds = %if.else, %if.then27
-//         //   %25 = load i8, i8* @num_connections, align 1
-//         //   %inc = add i8 %25, 1
-//         //   store i8 %inc, i8* @num_connections, align 1
-//         //   store i8 1, i8* %retval, align 1
-//         //   br label %return
+        // if.end41:                                         ; preds = %if.else, %if.then27
+        //   %25 = load i8, i8* @num_connections, align 1
+        //   %inc = add i8 %25, 1
+        //   store i8 %inc, i8* @num_connections, align 1
+        //   store i8 1, i8* %retval, align 1
+        //   br label %return
 
-//         // return:                                           ; preds = %if.end41, %if.then19
-//         //   %26 = load i8, i8* %retval, align 1
-//         //   ret i8 %26
+        // return:                                           ; preds = %if.end41, %if.then19
+        //   %26 = load i8, i8* %retval, align 1
+        //   ret i8 %26
 
-//     Block([prefixCode(),patch_block,postfixCode()])
-// }
+    [prefixCode(),patch_block,postfixCode()]
+}
 
 // function challenge_8_transport_handler_create_conn_mergerd_simple(patched:bool):codeRe {
     
@@ -305,10 +400,10 @@ function postfixCode():code{
 //     // assert vuln.block[2] == patch.block[2];
 // }
 
-//     function delete_connection():codeSeq
-//     {
-//         [CNil]
-//     }
+    function delete_connection():seq<Code>
+    {
+        [CNil]
+    }
 
     predicate validStartingState(s:state)
         // requires ValidState(s)
@@ -356,13 +451,13 @@ function postfixCode():code{
         && s.lvs["var_size_addr"] == (Int(0,IntType(1,false)))
         && s.lvs["var_conv16"] == (Int(0,IntType(1,false)))
         && s.lvs["var_div"] == (Int(0,IntType(1,false)))
-        && s.lvs["var_cmp17"] == (Int(0,IntType(1,false)))
+        && s.lvs["var_cmp17"] == (Int(0,IntType(1,true)))
         && s.lvs["var_call20"] == (Int(0,IntType(1,false)))
         && s.lvs["var_retval"] == (Ptr(0,0,0,1))
         && s.lvs["var_26"] == (Int(0,IntType(1,false)))
         && s.m.mem[0][0].mb? 
         && s.m.mem[0][0].size == 1
-        && !s.lvs["var_num_packets"].itype.signed
+        && s.lvs["var_num_packets"].itype.signed
         && s.lvs["var_num_packets"].itype.size == 4
         && s.lvs["var_num_packets"].val >= 0 
         && s.lvs["var_num_packets"].val < 0x10000
